this is better.

readvar/readvar.v
@@ -16,34 +16,101 @@ Module StringMapFacts := FMapFacts.WFacts_fun String_as_OT StringMap.
 
 Inductive var (t: Type): Type := mkvar (name : string): var t.
 
-Inductive value: Type := mkvalue (t: Type) (x : var t) (a : t): value.
+Inductive value: Type := mkvalue (t: Type) (a : t): value.
 
 Definition localenv := StringMap.t value.
 
-Definition localenv_sound (env: localenv): Prop :=
-   forall t name x, exists a,
-      x = mkvar t name ->
-      StringMap.find name env = Some (mkvalue t x a).
+Inductive program: Type :=
+| Something: program
+| UseVar: forall t, var t -> program
+| Block: list program -> program
+.
+Inductive in_program: forall t, var t -> program -> Prop :=
+| InProgVar: forall t name, in_program t (mkvar t name) (UseVar t (mkvar t name))
+| InProgBlockConsEq: forall t v p ps, in_program t v p -> in_program t v (Block (p :: ps))
+| InProgBlockConsNeq: forall t v p ps, in_program t v (Block ps) -> in_program t v (Block (p :: ps))
+.
 
-Lemma foo t t':
-   forall env name x,
-      localenv_sound env ->
-      x = mkvar t name ->
-      t = t'.
+Definition localenv_sound (env: localenv) (prog : program): Prop :=
+   forall t name, exists a,
+      in_program t (mkvar t name) prog ->
+       (StringMap.find name env = Some (mkvalue t a)) /\
+       (forall t', in_program t' (mkvar t' name) prog -> t = t').
+
+Lemma localenv_weaken (env: localenv) (prog: program):
+   forall (t : Type) name,
+      localenv_sound env prog ->
+      in_program t (mkvar t name) prog ->
+      StringMap.find name env = None -> False.
 Proof.
    intros.
    unfold localenv_sound in H.
-   remember H as H'; clear HeqH'.
-   specialize H with (t := t) (name := name) (x := mkvar t name).
-   specialize H' with (t := t') (name := name) (x := mkvar t' name).
-   destruct H as [a H]; destruct H' as [a' H'].
-   assert (mkvar t name = mkvar t name) as H1 by auto.
-   assert (mkvar t' name = mkvar t' name) as H1' by auto.
-   apply H in H1.
-   apply H' in H1'.
-   rewrite H1' in H1.
+   specialize H with (t := t) (name := name).
+   destruct H as [a H].
+   apply H in H0.
+   destruct H0 as [H0 _].
+   rewrite H1 in H0.
+   discriminate.
+Qed.
+
+Lemma localenv_weaken2 (env: localenv) (prog: program):
+   forall (t : Type) name,
+      localenv_sound env prog ->
+      in_program t (mkvar t name) prog ->
+      (forall t' a, StringMap.find name env = Some (mkvalue t' a) -> t' = t).
+Proof.
+   intros.
+   unfold localenv_sound in H.
+   specialize H with (t := t) (name := name).
+   destruct H as [a' H].
+   apply H in H0.
+   destruct H0 as [H0 _].
+   rewrite H1 in H0.
    congruence.
 Admitted.
+
+Lemma read_some:
+   forall t env prog name,
+      localenv_sound env prog ->
+      in_program t (mkvar t name) prog ->
+      exists v, StringMap.find name env = Some v.
+Proof.
+   intros.
+   induction H with (t := t) (name := name).
+   - apply H1 in H0.
+     destruct H0 as [H0 H2].
+     exists (mkvalue t x).
+     auto.
+Qed.
+
+(*
+Lemma foo (t : Type) (t' : Type):
+   forall env prog (name : string),
+      localenv_sound env prog ->
+      in_program t (mkvar t name) prog ->
+      t = t'.
+Proof.
+   intros env prog name S IN.
+   assert (exists v, StringMap.find name env = Some v).
+   apply read_some with (t := t) (prog := prog); auto.
+   destruct H as [v H].
+   destruct v.
+   unfold localenv_sound in S.
+   specialize S with (t := t') (name := name).
+   destruct S as [a' S].
+   apply S in IN.
+
+   unfold localenv_sound in S.
+   remember S as S'; clear HeqS'.
+   specialize S with (t := t) (name := name).
+   specialize S' with (t := t') (name := name).
+   destruct S as [a S]; destruct S' as [a' S'].
+   apply S in IN.
+   apply S' in IN'.
+   rewrite IN' in IN.
+   congruence.
+Admitted.
+*)
 
 Definition launder (t1 t2: Type) (x : t1) (k: t1 = t2): t2.
 Proof.
@@ -51,15 +118,25 @@ Proof.
    auto.
 Qed.
 
-Definition read {t} {hint: t} (x: var t) (env: localenv) (P: localenv_sound env): option t.
-destruct x.
-   refine (
-      match StringMap.find name env with
-      | Some (mkvalue t' (mkvar _ name') a) => Some (launder t' t a _)
-      | None => None
-      end
-   ).
+Definition read {t} (x: var t)
+                (env: localenv) (prog: program)
+                (P: localenv_sound env prog)
+                (P1: in_program t x prog)
+           : option t.
 Proof.
-apply (foo t' t env name (mkvar t' name)); auto.
+   destruct x.
+   remember (StringMap.find name env) as Q.
+   destruct Q.
+   - destruct v.
+     assert (t0 = t).
+     * apply (localenv_weaken2 env prog)
+          with (t := t) (name := name) (t' := t0) (a := a); auto.
+     * clear HeqQ.
+       rewrite H in a.
+       refine (Some a).
+   - symmetry in HeqQ.
+     apply localenv_weaken with (t := t) (name := name) in P; auto.
+     contradiction.
 Defined.
 Check read.
+
